src/util/MonadPlus.v
@@ -1,0 +1,12 @@
+Require Import riscv.util.Monad.
+
+(* Monad which also supports failure (mzero) and choice (mplus), typically used to chose
+   the first successful one *)
+Class MonadPlus(M: Type -> Type){MM: Monad M} := mkMonadPlus {
+  mzero: forall {A}, M A;
+  mplus: forall {A}, M A -> M A -> M A;
+
+  mzero_left: forall {A} (f: A -> M A), Bind mzero f = mzero;
+  mzero_right: forall {A B} (v: M A), Bind v (fun (_: A) => @mzero B) = @mzero B;
+  mplus_assoc: forall {A} (m1 m2 m3: M A), mplus m1 (mplus m2 m3) = mplus (mplus m1 m2) m3;
+}.
